isabelle/core/CoreTyEnvWellFormed.thy
@@ -7,11 +7,6 @@ definition tyenv_vars_well_kinded :: "CoreTyEnv \<Rightarrow> bool" where
   "tyenv_vars_well_kinded env =
     (\<forall>name ty. fmlookup (TE_TermVars env) name = Some ty \<longrightarrow> is_well_kinded env ty)"
 
-(* All term variables' types are ground (no metavariables) *)
-definition tyenv_vars_ground :: "CoreTyEnv \<Rightarrow> bool" where
-  "tyenv_vars_ground env =
-    (\<forall>name ty. fmlookup (TE_TermVars env) name = Some ty \<longrightarrow> is_ground ty)"
-
 (* All nonghost term variables' types are runtime types *)
 definition tyenv_vars_runtime :: "CoreTyEnv \<Rightarrow> bool" where
   "tyenv_vars_runtime env =
@@ -24,6 +19,11 @@ definition tyenv_ghost_vars_subset :: "CoreTyEnv \<Rightarrow> bool" where
   "tyenv_ghost_vars_subset env =
     (TE_GhostVars env |\<subseteq>| fmdom (TE_TermVars env))"
 
+(* The return type is well-kinded *)
+definition tyenv_return_type_well_kinded :: "CoreTyEnv \<Rightarrow> bool" where
+  "tyenv_return_type_well_kinded env =
+    is_well_kinded env (TE_ReturnType env)"
+
 (* Data constructors are consistent with datatypes:
    For each ctor in TE_DataCtors mapping to (dtName, tyArgMetavars, payload),
    dtName must be in TE_Datatypes with matching numTyArgs *)
@@ -33,28 +33,21 @@ definition tyenv_ctors_consistent :: "CoreTyEnv \<Rightarrow> bool" where
       fmlookup (TE_DataCtors env) ctorName = Some (dtName, tyArgMetavars, payload) \<longrightarrow>
       fmlookup (TE_Datatypes env) dtName = Some (length tyArgMetavars))"
 
-(* Data constructor payload types are well-kinded *)
+(* Data constructor payload types are well-kinded, in an appropriate env. *)
+(* (Note that well-kindedness depends only on TE_Datatypes and TE_TypeVars, so overriding
+   only TE_TypeVars is appropriate here.) *)
 definition tyenv_payloads_well_kinded :: "CoreTyEnv \<Rightarrow> bool" where
   "tyenv_payloads_well_kinded env =
     (\<forall>ctorName dtName tyArgMetavars payload.
       fmlookup (TE_DataCtors env) ctorName = Some (dtName, tyArgMetavars, payload) \<longrightarrow>
-      is_well_kinded env payload)"
+      is_well_kinded (env \<lparr> TE_TypeVars := fset_of_list tyArgMetavars \<rparr>) payload)"
 
-(* Metavars in data constructor payload types are a subset of the stated metavars *)
-(* (This means that after substituting in the actual type arguments, the payload will
-   have a ground type) *)
-definition tyenv_payloads_have_expected_metavars :: "CoreTyEnv \<Rightarrow> bool" where
-  "tyenv_payloads_have_expected_metavars env =
-    (\<forall>ctorName dtName tyArgMetavars payload.
-      fmlookup (TE_DataCtors env) ctorName = Some (dtName, tyArgMetavars, payload) \<longrightarrow>
-      type_metavars payload \<subseteq> set tyArgMetavars)"
-
-(* Data constructor type arguments (metavars) are distinct *)
-definition tyenv_ctor_metavars_distinct :: "CoreTyEnv \<Rightarrow> bool" where
-  "tyenv_ctor_metavars_distinct env =
-    (\<forall>ctorName dtName tyArgMetavars payload.
-      fmlookup (TE_DataCtors env) ctorName = Some (dtName, tyArgMetavars, payload) \<longrightarrow>
-      distinct tyArgMetavars)"
+(* Data constructor type arguments (type variables) are distinct *)
+definition tyenv_ctor_tyvars_distinct :: "CoreTyEnv \<Rightarrow> bool" where
+  "tyenv_ctor_tyvars_distinct env =
+    (\<forall>ctorName dtName tyVars payload.
+      fmlookup (TE_DataCtors env) ctorName = Some (dtName, tyVars, payload) \<longrightarrow>
+      distinct tyVars)"
 
 (* TE_DataCtorsByType is consistent with TE_DataCtors:
    A constructor is in TE_DataCtorsByType[dtName] iff it maps to dtName in TE_DataCtors *)
@@ -65,42 +58,40 @@ definition tyenv_ctors_by_type_consistent :: "CoreTyEnv \<Rightarrow> bool" wher
         (\<exists>tyArgMetavars payload.
           fmlookup (TE_DataCtors env) ctorName = Some (dtName, tyArgMetavars, payload))))"
 
-(* Function arg and return types are well-kinded *)
+(* Function arg and return types are well-kinded in an appropriate env. *)
 definition tyenv_fun_types_well_kinded :: "CoreTyEnv \<Rightarrow> bool" where
   "tyenv_fun_types_well_kinded env =
     (\<forall>funName info. fmlookup (TE_Functions env) funName = Some info \<longrightarrow>
-      (\<forall>ty \<in> fst ` set (FI_TmArgs info). is_well_kinded env ty) \<and>
-      is_well_kinded env (FI_ReturnType info))"
+      (\<forall>ty \<in> fst ` set (FI_TmArgs info).
+          is_well_kinded (env \<lparr> TE_TypeVars := fset_of_list (FI_TyArgs info) \<rparr>) ty) \<and>
+      is_well_kinded (env \<lparr> TE_TypeVars := fset_of_list (FI_TyArgs info) \<rparr>) (FI_ReturnType info))"
 
-(* Function arg and return types have the expected metavars *)
-definition tyenv_funs_have_expected_metavars :: "CoreTyEnv \<Rightarrow> bool" where
-  "tyenv_funs_have_expected_metavars env =
-    (\<forall>funName info. fmlookup (TE_Functions env) funName = Some info \<longrightarrow>
-      (\<forall>ty \<in> fst ` set (FI_TmArgs info). type_metavars ty \<subseteq> set (FI_TyArgs info)) \<and>
-      type_metavars (FI_ReturnType info) \<subseteq> set (FI_TyArgs info))"
-
-(* Function type arguments (metavars) are distinct *)
-definition tyenv_fun_metavars_distinct :: "CoreTyEnv \<Rightarrow> bool" where
-  "tyenv_fun_metavars_distinct env =
+(* Function type arguments (tyvars) are distinct *)
+definition tyenv_fun_tyvars_distinct :: "CoreTyEnv \<Rightarrow> bool" where
+  "tyenv_fun_tyvars_distinct env =
     (\<forall>funName info. fmlookup (TE_Functions env) funName = Some info \<longrightarrow>
       distinct (FI_TyArgs info))"
 
-(* For non-ghost functions, types must be runtime types *)
+(* For non-ghost functions, types must be runtime types (for polymorphic functions,
+   this only needs to hold when the type arguments themselves are runtime types). *)
 definition tyenv_fun_ghost_constraint :: "CoreTyEnv \<Rightarrow> bool" where
   "tyenv_fun_ghost_constraint env =
     (\<forall>funName info. fmlookup (TE_Functions env) funName = Some info \<and>
     (FI_Ghost info) = NotGhost \<longrightarrow>
-      (\<forall>ty \<in> fst ` set (FI_TmArgs info). is_runtime_type env ty) \<and>
-      is_runtime_type env (FI_ReturnType info))"
+      (let fenv = env \<lparr> TE_TypeVars := fset_of_list (FI_TyArgs info),
+                         TE_RuntimeTypeVars := fset_of_list (FI_TyArgs info) \<rparr>
+       in (\<forall>ty \<in> fst ` set (FI_TmArgs info). is_runtime_type fenv ty) \<and>
+          is_runtime_type fenv (FI_ReturnType info)))"
 
 (* For non-ghost datatypes, all constructor payload types must be runtime.
    This ensures variant types can be represented in memory (e.g. as tagged unions). *)
 definition tyenv_nonghost_payloads_runtime :: "CoreTyEnv \<Rightarrow> bool" where
   "tyenv_nonghost_payloads_runtime env =
-    (\<forall>ctorName dtName metavars payload.
-      fmlookup (TE_DataCtors env) ctorName = Some (dtName, metavars, payload) \<longrightarrow>
+    (\<forall>ctorName dtName tyVars payload.
+      fmlookup (TE_DataCtors env) ctorName = Some (dtName, tyVars, payload) \<longrightarrow>
       dtName |\<notin>| TE_GhostDatatypes env \<longrightarrow>
-      is_runtime_type env payload)"
+      is_runtime_type (env \<lparr> TE_TypeVars := fset_of_list tyVars,
+                              TE_RuntimeTypeVars := fset_of_list tyVars \<rparr>) payload)"
 
 (* Ghost datatypes must be a subset of all datatypes *)
 definition tyenv_ghost_datatypes_subset :: "CoreTyEnv \<Rightarrow> bool" where
@@ -111,17 +102,15 @@ definition tyenv_ghost_datatypes_subset :: "CoreTyEnv \<Rightarrow> bool" where
 definition tyenv_well_formed :: "CoreTyEnv \<Rightarrow> bool" where
   "tyenv_well_formed env =
     (tyenv_vars_well_kinded env \<and>
-     tyenv_vars_ground env \<and>
      tyenv_vars_runtime env \<and>
      tyenv_ghost_vars_subset env \<and>
+     tyenv_return_type_well_kinded env \<and>
      tyenv_ctors_consistent env \<and>
      tyenv_payloads_well_kinded env \<and>
-     tyenv_payloads_have_expected_metavars env \<and>
-     tyenv_ctor_metavars_distinct env \<and>
+     tyenv_ctor_tyvars_distinct env \<and>
      tyenv_ctors_by_type_consistent env \<and>
      tyenv_fun_types_well_kinded env \<and>
-     tyenv_funs_have_expected_metavars env \<and>
-     tyenv_fun_metavars_distinct env \<and>
+     tyenv_fun_tyvars_distinct env \<and>
      tyenv_fun_ghost_constraint env \<and>
      tyenv_nonghost_payloads_runtime env \<and>
      tyenv_ghost_datatypes_subset env)"
@@ -130,23 +119,19 @@ definition tyenv_well_formed :: "CoreTyEnv \<Rightarrow> bool" where
 lemma tyenv_well_formed_add_var:
   assumes wf: "tyenv_well_formed env"
     and ty_wk: "is_well_kinded env ty"
-    and ty_ground: "is_ground ty"
     and ty_runtime: "is_runtime_type env ty"
   shows "tyenv_well_formed (env \<lparr> TE_TermVars := fmupd var ty (TE_TermVars env) \<rparr>)"
 proof -
   let ?env' = "env \<lparr> TE_TermVars := fmupd var ty (TE_TermVars env) \<rparr>"
   from wf have wk: "tyenv_vars_well_kinded env"
-    and gr: "tyenv_vars_ground env"
     and rt: "tyenv_vars_runtime env"
     and gvs: "tyenv_ghost_vars_subset env"
     and rest: "tyenv_ctors_consistent env"
               "tyenv_payloads_well_kinded env"
-              "tyenv_payloads_have_expected_metavars env"
-              "tyenv_ctor_metavars_distinct env"
+              "tyenv_ctor_tyvars_distinct env"
               "tyenv_ctors_by_type_consistent env"
               "tyenv_fun_types_well_kinded env"
-              "tyenv_funs_have_expected_metavars env"
-              "tyenv_fun_metavars_distinct env"
+              "tyenv_fun_tyvars_distinct env"
               "tyenv_fun_ghost_constraint env"
               "tyenv_nonghost_payloads_runtime env"
               "tyenv_ghost_datatypes_subset env"
@@ -168,62 +153,74 @@ proof -
   have "tyenv_vars_well_kinded ?env'"
     using wk ty_wk unfolding tyenv_vars_well_kinded_def
     by (auto simp: wk_preserved split: if_splits)
-  moreover have "tyenv_vars_ground ?env'"
-    using gr ty_ground unfolding tyenv_vars_ground_def
-    by (auto split: if_splits)
   moreover have "tyenv_vars_runtime ?env'"
     using rt ty_runtime unfolding tyenv_vars_runtime_def
     by (auto simp: rt_preserved split: if_splits)
   moreover have "tyenv_ghost_vars_subset ?env'"
     using gvs unfolding tyenv_ghost_vars_subset_def by auto
+  moreover have "tyenv_return_type_well_kinded ?env'"
+    using local.wf tyenv_return_type_well_kinded_def tyenv_well_formed_def wk_preserved
+    by auto
   moreover have "tyenv_ctors_consistent ?env'" using rest(1)
     unfolding tyenv_ctors_consistent_def by simp
-  moreover have "tyenv_payloads_well_kinded ?env'" using rest(2)
-    unfolding tyenv_payloads_well_kinded_def by (simp add: wk_preserved)
-  moreover have "tyenv_payloads_have_expected_metavars ?env'" using rest(3)
-    unfolding tyenv_payloads_have_expected_metavars_def by simp
-  moreover have "tyenv_ctor_metavars_distinct ?env'" using rest(4)
-    unfolding tyenv_ctor_metavars_distinct_def by simp
-  moreover have "tyenv_ctors_by_type_consistent ?env'" using rest(5)
+  moreover have "tyenv_payloads_well_kinded ?env'"
+  proof -
+    have "\<And>mvs t. is_well_kinded (?env' \<lparr> TE_TypeVars := fset_of_list mvs \<rparr>) t =
+                    is_well_kinded (env \<lparr> TE_TypeVars := fset_of_list mvs \<rparr>) t"
+      by (rule is_well_kinded_cong_env) simp_all
+    thus ?thesis using rest(2) unfolding tyenv_payloads_well_kinded_def by simp
+  qed
+  moreover have "tyenv_ctor_tyvars_distinct ?env'" using rest(3)
+    unfolding tyenv_ctor_tyvars_distinct_def by simp
+  moreover have "tyenv_ctors_by_type_consistent ?env'" using rest(4)
     unfolding tyenv_ctors_by_type_consistent_def by simp
-  moreover have "tyenv_fun_types_well_kinded ?env'" using rest(6)
-    unfolding tyenv_fun_types_well_kinded_def by (simp add: wk_preserved)
-  moreover have "tyenv_funs_have_expected_metavars ?env'" using rest(7)
-    unfolding tyenv_funs_have_expected_metavars_def by simp
-  moreover have "tyenv_fun_metavars_distinct ?env'" using rest(8)
-    unfolding tyenv_fun_metavars_distinct_def by simp
-  moreover have "tyenv_fun_ghost_constraint ?env'" using rest(9)
-    unfolding tyenv_fun_ghost_constraint_def by (auto simp: rt_preserved)
-  moreover have "tyenv_nonghost_payloads_runtime ?env'" using rest(10)
-    unfolding tyenv_nonghost_payloads_runtime_def by (simp add: rt_preserved)
-  moreover have "tyenv_ghost_datatypes_subset ?env'" using rest(11)
+  moreover have "tyenv_fun_types_well_kinded ?env'"
+  proof -
+    have "\<And>tvs t. is_well_kinded (?env' \<lparr> TE_TypeVars := tvs \<rparr>) t =
+                    is_well_kinded (env \<lparr> TE_TypeVars := tvs \<rparr>) t"
+      by (rule is_well_kinded_cong_env) simp_all
+    thus ?thesis using rest(5) unfolding tyenv_fun_types_well_kinded_def by simp
+  qed
+  moreover have "tyenv_fun_tyvars_distinct ?env'" using rest(6)
+    unfolding tyenv_fun_tyvars_distinct_def by simp
+  moreover have "tyenv_fun_ghost_constraint ?env'"
+  proof -
+    have "\<And>rtvs tvs t. is_runtime_type (?env' \<lparr> TE_TypeVars := tvs, TE_RuntimeTypeVars := rtvs \<rparr>) t =
+                        is_runtime_type (env \<lparr> TE_TypeVars := tvs, TE_RuntimeTypeVars := rtvs \<rparr>) t"
+      by (rule is_runtime_type_cong_env) simp_all
+    thus ?thesis using rest(7) unfolding tyenv_fun_ghost_constraint_def Let_def by simp
+  qed
+  moreover have "tyenv_nonghost_payloads_runtime ?env'"
+  proof -
+    have "\<And>tvs rtvs t. is_runtime_type (?env' \<lparr> TE_TypeVars := tvs, TE_RuntimeTypeVars := rtvs \<rparr>) t =
+                        is_runtime_type (env \<lparr> TE_TypeVars := tvs, TE_RuntimeTypeVars := rtvs \<rparr>) t"
+      by (rule is_runtime_type_cong_env) simp_all
+    thus ?thesis using rest(8) unfolding tyenv_nonghost_payloads_runtime_def by simp
+  qed
+  moreover have "tyenv_ghost_datatypes_subset ?env'" using rest(9)
     unfolding tyenv_ghost_datatypes_subset_def by simp
   ultimately show ?thesis unfolding tyenv_well_formed_def by auto
 qed
 
-(* Adding a well-kinded, ground ghost variable preserves tyenv_well_formed.
+(* Adding a well-kinded ghost variable preserves tyenv_well_formed.
    Ghost variables do not need to be runtime types. *)
 lemma tyenv_well_formed_add_ghost_var:
   assumes wf: "tyenv_well_formed env"
     and ty_wk: "is_well_kinded env ty"
-    and ty_ground: "is_ground ty"
   shows "tyenv_well_formed (env \<lparr> TE_TermVars := fmupd var ty (TE_TermVars env),
                                  TE_GhostVars := finsert var (TE_GhostVars env) \<rparr>)"
 proof -
   let ?env' = "env \<lparr> TE_TermVars := fmupd var ty (TE_TermVars env),
                      TE_GhostVars := finsert var (TE_GhostVars env) \<rparr>"
   from wf have wk: "tyenv_vars_well_kinded env"
-    and gr: "tyenv_vars_ground env"
     and rt: "tyenv_vars_runtime env"
     and gvs: "tyenv_ghost_vars_subset env"
     and rest: "tyenv_ctors_consistent env"
               "tyenv_payloads_well_kinded env"
-              "tyenv_payloads_have_expected_metavars env"
-              "tyenv_ctor_metavars_distinct env"
+              "tyenv_ctor_tyvars_distinct env"
               "tyenv_ctors_by_type_consistent env"
               "tyenv_fun_types_well_kinded env"
-              "tyenv_funs_have_expected_metavars env"
-              "tyenv_fun_metavars_distinct env"
+              "tyenv_fun_tyvars_distinct env"
               "tyenv_fun_ghost_constraint env"
               "tyenv_nonghost_payloads_runtime env"
               "tyenv_ghost_datatypes_subset env"
@@ -244,35 +241,51 @@ proof -
   have "tyenv_vars_well_kinded ?env'"
     using wk ty_wk unfolding tyenv_vars_well_kinded_def
     by (auto simp: wk_preserved split: if_splits)
-  moreover have "tyenv_vars_ground ?env'"
-    using gr ty_ground unfolding tyenv_vars_ground_def
-    by (auto split: if_splits)
   moreover have "tyenv_vars_runtime ?env'"
     using rt unfolding tyenv_vars_runtime_def
     by (auto simp: rt_preserved split: if_splits)
   moreover have "tyenv_ghost_vars_subset ?env'"
     using gvs unfolding tyenv_ghost_vars_subset_def by auto
+  moreover have "tyenv_return_type_well_kinded ?env'"
+    using local.wf tyenv_return_type_well_kinded_def tyenv_well_formed_def wk_preserved
+    by auto
   moreover have "tyenv_ctors_consistent ?env'" using rest(1)
     unfolding tyenv_ctors_consistent_def by simp
-  moreover have "tyenv_payloads_well_kinded ?env'" using rest(2)
-    unfolding tyenv_payloads_well_kinded_def by (simp add: wk_preserved)
-  moreover have "tyenv_payloads_have_expected_metavars ?env'" using rest(3)
-    unfolding tyenv_payloads_have_expected_metavars_def by simp
-  moreover have "tyenv_ctor_metavars_distinct ?env'" using rest(4)
-    unfolding tyenv_ctor_metavars_distinct_def by simp
-  moreover have "tyenv_ctors_by_type_consistent ?env'" using rest(5)
+  moreover have "tyenv_payloads_well_kinded ?env'"
+  proof -
+    have "\<And>mvs t. is_well_kinded (?env' \<lparr> TE_TypeVars := fset_of_list mvs \<rparr>) t =
+                    is_well_kinded (env \<lparr> TE_TypeVars := fset_of_list mvs \<rparr>) t"
+      by (rule is_well_kinded_cong_env) simp_all
+    thus ?thesis using rest(2) unfolding tyenv_payloads_well_kinded_def by simp
+  qed
+  moreover have "tyenv_ctor_tyvars_distinct ?env'" using rest(3)
+    unfolding tyenv_ctor_tyvars_distinct_def by simp
+  moreover have "tyenv_ctors_by_type_consistent ?env'" using rest(4)
     unfolding tyenv_ctors_by_type_consistent_def by simp
-  moreover have "tyenv_fun_types_well_kinded ?env'" using rest(6)
-    unfolding tyenv_fun_types_well_kinded_def by (simp add: wk_preserved)
-  moreover have "tyenv_funs_have_expected_metavars ?env'" using rest(7)
-    unfolding tyenv_funs_have_expected_metavars_def by simp
-  moreover have "tyenv_fun_metavars_distinct ?env'" using rest(8)
-    unfolding tyenv_fun_metavars_distinct_def by simp
-  moreover have "tyenv_fun_ghost_constraint ?env'" using rest(9)
-    unfolding tyenv_fun_ghost_constraint_def by (auto simp: rt_preserved)
-  moreover have "tyenv_nonghost_payloads_runtime ?env'" using rest(10)
-    unfolding tyenv_nonghost_payloads_runtime_def by (simp add: rt_preserved)
-  moreover have "tyenv_ghost_datatypes_subset ?env'" using rest(11)
+  moreover have "tyenv_fun_types_well_kinded ?env'"
+  proof -
+    have "\<And>tvs t. is_well_kinded (?env' \<lparr> TE_TypeVars := tvs \<rparr>) t =
+                    is_well_kinded (env \<lparr> TE_TypeVars := tvs \<rparr>) t"
+      by (rule is_well_kinded_cong_env) simp_all
+    thus ?thesis using rest(5) unfolding tyenv_fun_types_well_kinded_def by simp
+  qed
+  moreover have "tyenv_fun_tyvars_distinct ?env'" using rest(6)
+    unfolding tyenv_fun_tyvars_distinct_def by simp
+  moreover have "tyenv_fun_ghost_constraint ?env'"
+  proof -
+    have "\<And>rtvs tvs t. is_runtime_type (?env' \<lparr> TE_TypeVars := tvs, TE_RuntimeTypeVars := rtvs \<rparr>) t =
+                        is_runtime_type (env \<lparr> TE_TypeVars := tvs, TE_RuntimeTypeVars := rtvs \<rparr>) t"
+      by (rule is_runtime_type_cong_env) simp_all
+    thus ?thesis using rest(7) unfolding tyenv_fun_ghost_constraint_def Let_def by simp
+  qed
+  moreover have "tyenv_nonghost_payloads_runtime ?env'"
+  proof -
+    have "\<And>tvs rtvs t. is_runtime_type (?env' \<lparr> TE_TypeVars := tvs, TE_RuntimeTypeVars := rtvs \<rparr>) t =
+                        is_runtime_type (env \<lparr> TE_TypeVars := tvs, TE_RuntimeTypeVars := rtvs \<rparr>) t"
+      by (rule is_runtime_type_cong_env) simp_all
+    thus ?thesis using rest(8) unfolding tyenv_nonghost_payloads_runtime_def by simp
+  qed
+  moreover have "tyenv_ghost_datatypes_subset ?env'" using rest(9)
     unfolding tyenv_ghost_datatypes_subset_def by simp
   ultimately show ?thesis unfolding tyenv_well_formed_def by auto
 qed
@@ -287,15 +300,21 @@ proof -
     using is_well_kinded_cong_env[of ?env' env] by simp
   have rt: "\<And>ty. is_runtime_type ?env' ty = is_runtime_type env ty"
     using is_runtime_type_cong_env[of ?env' env] by simp
+  have scope_wk: "\<And>tvs t. is_well_kinded (?env' \<lparr> TE_TypeVars := tvs \<rparr>) t =
+                            is_well_kinded (env \<lparr> TE_TypeVars := tvs \<rparr>) t"
+    by (rule is_well_kinded_cong_env) simp_all
+  have scope_rt: "\<And>tvs rtvs t. is_runtime_type (?env' \<lparr> TE_TypeVars := tvs, TE_RuntimeTypeVars := rtvs \<rparr>) t =
+                                 is_runtime_type (env \<lparr> TE_TypeVars := tvs, TE_RuntimeTypeVars := rtvs \<rparr>) t"
+    by (rule is_runtime_type_cong_env) simp_all
   from assms show ?thesis unfolding tyenv_well_formed_def
-    tyenv_vars_well_kinded_def tyenv_vars_ground_def tyenv_vars_runtime_def
-    tyenv_ghost_vars_subset_def tyenv_ctors_consistent_def
-    tyenv_payloads_well_kinded_def tyenv_payloads_have_expected_metavars_def
-    tyenv_ctor_metavars_distinct_def tyenv_ctors_by_type_consistent_def
-    tyenv_fun_types_well_kinded_def tyenv_funs_have_expected_metavars_def
-    tyenv_fun_metavars_distinct_def tyenv_fun_ghost_constraint_def
+    tyenv_vars_well_kinded_def tyenv_vars_runtime_def
+    tyenv_ghost_vars_subset_def tyenv_return_type_well_kinded_def tyenv_ctors_consistent_def
+    tyenv_payloads_well_kinded_def
+    tyenv_ctor_tyvars_distinct_def tyenv_ctors_by_type_consistent_def
+    tyenv_fun_types_well_kinded_def
+    tyenv_fun_tyvars_distinct_def tyenv_fun_ghost_constraint_def Let_def
     tyenv_nonghost_payloads_runtime_def tyenv_ghost_datatypes_subset_def
-    by (auto simp: wk rt)
+    by (force simp: wk rt scope_wk scope_rt)
 qed
 
 end
