isabelle/core/CoreStmtTypecheck.thy
@@ -23,7 +23,6 @@ where
     (if fmlookup (TE_TermVars env) varName \<noteq> None then None  \<comment> \<open>no shadowing\<close>
      else if (ghost = Ghost \<longrightarrow> declGhost = Ghost)
         \<and> is_well_kinded env varTy
-        \<and> is_ground varTy
         \<and> (declGhost = NotGhost \<longrightarrow> is_runtime_type env varTy)
         \<and> core_term_type env declGhost initTm = Some varTy
      then Some (env \<lparr> TE_TermVars := fmupd varName varTy (TE_TermVars env),
@@ -124,13 +123,12 @@ using assms proof (cases stmt)
     case Var
     from assms CoreStmt_VarDecl Var obtain
       wk: "is_well_kinded env varTy" and
-      gr: "is_ground varTy" and
       rt: "declGhost = NotGhost \<longrightarrow> is_runtime_type env varTy"
       by (auto split: if_splits)
     show ?thesis proof (cases declGhost)
       case NotGhost
       from rt NotGhost have "is_runtime_type env varTy" by simp
-      from tyenv_well_formed_add_var[OF assms(2) wk gr this]
+      from tyenv_well_formed_add_var[OF assms(2) wk this]
       have wf': "tyenv_well_formed (env \<lparr> TE_TermVars := fmupd varName varTy (TE_TermVars env) \<rparr>)" .
       from assms CoreStmt_VarDecl Var NotGhost have env'_eq:
         "env' = env \<lparr> TE_TermVars := fmupd varName varTy (TE_TermVars env),
@@ -140,7 +138,7 @@ using assms proof (cases stmt)
       with wf' show ?thesis by simp
     next
       case Ghost
-      from tyenv_well_formed_add_ghost_var[OF assms(2) wk gr]
+      from tyenv_well_formed_add_ghost_var[OF assms(2) wk]
       have "tyenv_well_formed (env \<lparr> TE_TermVars := fmupd varName varTy (TE_TermVars env),
                                      TE_GhostVars := finsert varName (TE_GhostVars env) \<rparr>)" .
       with assms CoreStmt_VarDecl Var Ghost show ?thesis
